kindof working

leanTheories/StackComp/Comp.lean
@@ -4,4 +4,182 @@ import StackComp.ScLib
 
 namespace StackComp
 
+/-!
+Checking imports are working
+-- #check inst
+-- #check aexp
+-- #check binop
+-- #check List
+-/
+
+def comp_aexp (a : aexp) : (List inst) :=
+  match a with
+  | .ANum i       => [.Const i]
+  | .AId v        => [.Load v]
+  | .APlus a1 a2  => (comp_aexp a2) ++ (comp_aexp a1) ++ [(.Binop .B_Add)]
+  | .AMinus a1 a2 => (comp_aexp a2) ++ (comp_aexp a1) ++ [(.Binop .B_Minus)]
+  | .AMult a1 a2  => (comp_aexp a2) ++ (comp_aexp a1) ++ [(.Binop .B_Mult)]
+  | .ADiv a1 a2   => (comp_aexp a2) ++ (comp_aexp a1) ++ [(.Binop .B_Div)]
+
+def comp_com (c : com) : (List inst) := 
+  match c with
+  | .CAsgn x a  => (comp_aexp a) ++ [.Set x]
+  | .CSeq c1 c2 => (comp_com c1) ++ (comp_com c2)
+
+/-! Testing compilation -/
+-- #eval comp_aexp (.APlus (.ANum 10) (.AId "x"))
+#eval comp_aexp (.ADiv (.ANum 9) (.ANum 3))
+#eval aeval empty_state (.ADiv (.ANum 9) (.ANum 3))
+-- (.ADiv 80 10)
+-- ==> .ADiv a1 a2
+-- ==> [const 10, const 80, binop b_div]
+-- ==> [const a2, const a1, binop b_div]
+-- #eval comp_com (.CAsgn "x" (.APlus (.ANum 10) (.ANum 3)))
+
+theorem seval_append {is1 is2 s1 st1 s2 st2 s3 st3} :
+  seval is1 (s1, st1) (s2, st2) →
+  seval is2 (s2, st2) (s3, st3) →
+  seval (is1 ++ is2) (s1, st1) (s3, st3) :=
+  by
+    intros h1 h2
+    cases h1
+    case NilI =>
+        exact h2
+    case ConsI i is s1' st1' hi hs =>
+        apply seval.ConsI
+        exact hi
+        apply seval_append
+        exact hs
+        apply h2
+
+/-! Proving stages of compilation correct -/
+theorem comp_aexp_cert {a st i}:
+  aeval st a = i →
+  seval (comp_aexp a) (s, st) (i::s, st) :=
+  by
+    induction a generalizing i s with
+    | ANum i' =>
+      intro h
+      rw [aeval] at h
+      rw [comp_aexp]
+      rw [h]
+      apply seval.ConsI
+      apply ieval.I_Const
+      apply seval.NilI
+    | AId x =>
+      intro h
+      rw [aeval] at h
+      rw[comp_aexp]
+      apply seval.ConsI
+      apply ieval.I_Load
+      rw [h]
+      apply seval.NilI
+    | APlus a1 a2 ha1 ha2 =>
+      intro h
+      rw [aeval] at h
+      rw [comp_aexp]
+      let i1 := aeval st a1
+      let i2 := aeval st a2
+      have h1 : aeval st a1 = i1 := rfl
+      have h2 : aeval st a2 = i2 := rfl
+      rw [h1, h2] at h
+      have eval_a2 : seval (comp_aexp a2) (s, st) (i2 :: s, st) := ha2 h2
+      have eval_a1 : seval (comp_aexp a1) (i2 :: s, st) (i1 :: i2 :: s, st) := by 
+        apply ha1
+        apply h1
+      have eval_a1_a2 : seval (comp_aexp a2 ++ comp_aexp a1) (s, st) (i1 :: i2 :: s, st) := by
+        apply seval_append
+        exact eval_a2
+        apply eval_a1
+      apply seval_append
+      exact eval_a1_a2
+      apply seval.ConsI
+      apply ieval.I_Binop
+      rw [←h]
+      rw [bo_eval]
+      simp
+      apply seval.NilI
+    | AMinus a1 a2 ha1 ha2 =>
+      intro h
+      rw [aeval] at h
+      rw [comp_aexp]
+      let i1 := aeval st a1
+      let i2 := aeval st a2
+      have h1 : aeval st a1 = i1 := rfl
+      have h2 : aeval st a2 = i2 := rfl
+      rw [h1, h2] at h
+      have eval_a2 : seval (comp_aexp a2) (s, st) (i2 :: s, st) := ha2 h2
+      have eval_a1 : seval (comp_aexp a1) (i2 :: s, st) (i1 :: i2 :: s, st) := by 
+        apply ha1
+        apply h1
+      have eval_a1_a2 : seval (comp_aexp a2 ++ comp_aexp a1) (s, st) (i1 :: i2 :: s, st) := by
+        apply seval_append
+        exact eval_a2
+        apply eval_a1
+      apply seval_append
+      exact eval_a1_a2
+      apply seval.ConsI
+      apply ieval.I_Binop
+      rw [←h]
+      rw [bo_eval]
+      simp
+      apply seval.NilI
+    | AMult a1 a2 ha1 ha2 =>
+      intro h
+      rw [aeval] at h
+      rw [comp_aexp]
+      let i1 := aeval st a1
+      let i2 := aeval st a2
+      have h1 : aeval st a1 = i1 := rfl
+      have h2 : aeval st a2 = i2 := rfl
+      rw [h1, h2] at h
+      have eval_a2 : seval (comp_aexp a2) (s, st) (i2 :: s, st) := ha2 h2
+      have eval_a1 : seval (comp_aexp a1) (i2 :: s, st) (i1 :: i2 :: s, st) := by 
+        apply ha1
+        apply h1
+      have eval_a1_a2 : seval (comp_aexp a2 ++ comp_aexp a1) (s, st) (i1 :: i2 :: s, st) := by
+        apply seval_append
+        exact eval_a2
+        apply eval_a1
+      apply seval_append
+      exact eval_a1_a2
+      apply seval.ConsI
+      apply ieval.I_Binop
+      rw [←h]
+      rw [bo_eval]
+      simp
+      apply seval.NilI
+    | ADiv a1 a2 ha1 ha2 =>
+      intro h
+      rw [aeval] at h
+      rw [comp_aexp]
+      let i1 := aeval st a1
+      let i2 := aeval st a2
+      have h1 : aeval st a1 = i1 := rfl
+      have h2 : aeval st a2 = i2 := rfl
+      rw [h1, h2] at h
+      have eval_a2 : seval (comp_aexp a2) (s, st) (i2 :: s, st) := ha2 h2
+      have eval_a1 : seval (comp_aexp a1) (i2 :: s, st) (i1 :: i2 :: s, st) := by 
+        apply ha1
+        apply h1
+      have eval_a1_a2 : seval (comp_aexp a2 ++ comp_aexp a1) (s, st) (i1 :: i2 :: s, st) := by
+        apply seval_append
+        exact eval_a2
+        apply eval_a1
+      apply seval_append
+      exact eval_a1_a2
+      apply seval.ConsI
+      apply ieval.I_Binop
+      rw [←h]
+      rw [bo_eval]
+      simp
+      apply seval.NilI
+
+theorem comp_state_cert {c s st st1 st2}
+  (hl : ceval c st st1)
+  (hr : seval (comp_com c) (empty_stack, st) (s, st2)):
+  st1 = st2 :=
+  by
+    sorry
+
 end StackComp
